Nominal-Utils.thy
@@ -116,5 +116,12 @@ lemma fresh_star_append:
   shows "a \<sharp>* (xs @ ys) \<longleftrightarrow> a \<sharp>* xs \<and> a \<sharp>* ys"
 by (metis fresh_star_def fresh_append)
 
+lemma fresh_list_elem:
+  assumes "a \<sharp> \<Gamma>"
+  and "e \<in> set \<Gamma>"
+  shows "a \<sharp> e"
+using assms
+by(induct \<Gamma>)(auto simp add: fresh_Cons)
+
 
 end
